Add jellyfish code and val_rep

lib/node_rep.v
@@ -2,20 +2,32 @@ From iris.heap_lang Require Import notation.
 
 Local Open Scope Z.
 
-Definition node_rep : Type := Z * loc * option loc * val.
+Definition val_rep : Type := Z * val * loc.
 
-Definition node_key (n: node_rep) : Z := n.1.1.1.
+Definition val_ts (v: val_rep) : Z := v.1.1.
+Definition val_v (v: val_rep) : val := v.1.2.
+Definition val_next (v: val_rep) : loc := v.2.
+
+Definition valTs : val := λ: "l", Fst (Fst "l").
+Definition valV : val := λ: "l", Snd (Fst "l").
+Definition valNext : val := λ: "l", Snd "l".
+
+Definition rep_to_val (v: val_rep) : val := 
+  (#(val_ts v), val_v v, #(val_next v)).
+
+Definition node_rep : Type := Z * loc * loc * option loc * val.
+
+Definition node_key (n: node_rep) : Z := n.1.1.1.1.
+Definition node_val (n: node_rep) : loc := n.1.1.1.2.
 Definition node_next (n: node_rep) : loc := n.1.1.2.
 Definition node_down (n: node_rep) : option loc := n.1.2.
 Definition node_lock (n: node_rep) : val := n.2.
 
-Definition nodeKey : val := λ: "l", Fst (Fst (Fst "l")).
+Definition nodeKey : val := λ: "l", Fst (Fst (Fst (Fst "l"))).
+Definition nodeVal : val := λ: "l", Snd (Fst (Fst (Fst "l"))).
 Definition nodeNext : val := λ: "l", Snd (Fst (Fst "l")).
 Definition nodeDown : val := λ: "l", Snd (Fst "l").
 Definition nodeLock : val := λ: "l", Snd "l".
-
-Definition dummy_null : loc := {|loc_car := 0|}.
-Definition dummy_lock : val := #().
 
 Definition oloc_to_val (ol: option loc) : val := 
   match ol with
@@ -24,21 +36,39 @@ Definition oloc_to_val (ol: option loc) : val :=
   end.
 
 Definition rep_to_node (n: node_rep) : val :=
-  (#(node_key n), #(node_next n), oloc_to_val (node_down n), (node_lock n)).
+  (#(node_key n), #(node_val n), #(node_next n), oloc_to_val (node_down n), (node_lock n)).
 
+Definition dummy_null : loc := {|loc_car := 0|}.
+Definition dummy_lock : val := #().
+
+
+Lemma fold_rep_to_val (v: val_rep) :
+  ((#(val_ts v), val_v v, #(val_next v)))%V =
+  rep_to_val v.
+Proof. done. Qed.
 
 Lemma fold_rep_to_node (n: node_rep) :
-  ((#(node_key n), #(node_next n), oloc_to_val (node_down n), (node_lock n)))%V =
+  ((#(node_key n), #(node_val n), #(node_next n), oloc_to_val (node_down n), (node_lock n)))%V =
   rep_to_node n.
 Proof. done. Qed.
+
+Lemma rep_to_val_inj rep rep' :
+  rep_to_val rep = rep_to_val rep' →
+  rep = rep'.
+Proof.
+  destruct rep as ((?&?)&?).
+  destruct rep' as ((?&?)&?).
+  rewrite /rep_to_val/val_ts/val_v/val_next/=.
+  intros; congruence.
+Qed.
 
 Lemma rep_to_node_inj rep rep':
   rep_to_node rep = rep_to_node rep' →
   rep = rep'.
 Proof.
-  destruct rep as (((?&?)&down)&?). 
-  destruct rep' as (((?&?)&down')&?).
-  rewrite /rep_to_node/node_key/node_next/node_down/node_lock//=.
+  destruct rep as ((((?&v)&?)&down)&?). 
+  destruct rep' as ((((?&v')&?)&down')&?).
+  rewrite /rep_to_node/node_key/node_val/node_next/node_down/node_lock//=.
   destruct down; destruct down'.
   all: inversion 1; congruence.
 Qed.
