lazy_list/spec/new.v
@@ -42,8 +42,8 @@ Module NewSpec (Params: LAZY_LIST_PARAMS).
 
       iIntros (l γ) "#Hlock".
       wp_pures; wp_alloc h as "Hh".
-      rewrite (fold_rep_to_node (INT_MIN, t, None, l)).
-      set (head := (INT_MIN, t, None, l)).
+      rewrite (fold_rep_to_node (INT_MIN, dummy_null, t, None, l)).
+      set (head := (INT_MIN, dummy_null, t, None, l)).
 
       set (Γ := mk_lazy_gname γauth γfrac γkeys).
       iMod (inv_alloc lazyN ⊤ (lazy_list_inv head Γ) 
